tidying the index

doc-src/TutorialI/Recdef/Induction.thy
@@ -48,7 +48,7 @@ definition of @{term"sep"}.
 In general, the format of invoking recursion induction is
 \begin{quote}
 \isacommand{apply}@{text"(induct_tac"} $x@1 \dots x@n$ @{text"rule:"} $f$@{text".induct)"}
-\end{quote}\index{*induct_tac}%
+\end{quote}\index{*induct_tac (method)}%
 where $x@1~\dots~x@n$ is a list of free variables in the subgoal and $f$ the
 name of a function that takes an $n$-tuple. Usually the subgoal will
 contain the term $f(x@1,\dots,x@n)$ but this need not be the case. The
