doc-src/TutorialI/Misc/Translations.thy
@@ -4,8 +4,10 @@ theory Translations = Main:
 subsection{*Syntax Translations*}
 
 text{*\label{sec:def-translations}
+\indexbold{syntax translations|(}%
+\indexbold{translations@\isacommand {translations} (command)|(}
 Isabelle offers an additional definition-like facility,
-\textbf{syntax translations}\indexbold{syntax translation}.
+\textbf{syntax translations}.
 They resemble macros: upon parsing, the defined concept is immediately
 replaced by its definition, and this is reversed upon printing. For example,
 the symbol @{text"\<noteq>"} is defined via a syntax translation:
@@ -13,7 +15,7 @@ the symbol @{text"\<noteq>"} is defined via a syntax translation:
 
 translations "x \<noteq> y" \<rightleftharpoons> "\<not>(x = y)"
 
-text{*\indexbold{*translations}\indexbold{$IsaEqTrans@\isasymrightleftharpoons}
+text{*\indexbold{$IsaEqTrans@\isasymrightleftharpoons}
 \noindent
 Internally, @{text"\<noteq>"} never appears.
 
@@ -27,7 +29,9 @@ crops up occasionally: a number of HOL's built-in constructs are defined
 via translations.  Translations are preferable to definitions when the new 
 concept is a trivial variation on an existing one.  For example, we
 don't need to derive new theorems about @{text"\<noteq>"}, since existing theorems
-about @{text"="} still apply.
+about @{text"="} still apply.%
+\indexbold{syntax translations|)}%
+\indexbold{translations@\isacommand {translations} (command)|)}
 *}
 
 (*<*)
