doc-src/TutorialI/Misc/types.thy
@@ -3,7 +3,7 @@ types number       = nat
       gate         = "bool \<Rightarrow> bool \<Rightarrow> bool"
       ('a,'b)alist = "('a \<times> 'b)list";
 
-text{*\noindent\indexbold{*types}%
+text{*\noindent
 Internally all synonyms are fully expanded.  As a consequence Isabelle's
 output never contains synonyms.  Their main purpose is to improve the
 readability of theories.  Synonyms can be used just like any other
@@ -15,7 +15,7 @@ consts nand :: gate
 
 subsection{*Constant Definitions*}
 
-text{*\label{sec:ConstDefinitions}\indexbold{definition}%
+text{*\label{sec:ConstDefinitions}\indexbold{definitions}%
 The above constants @{term"nand"} and @{term"xor"} are non-recursive and can
 therefore be defined directly by
 *}
@@ -24,11 +24,12 @@ defs nand_def: "nand A B \<equiv> \<not>(A \<and> B)"
      xor_def:  "xor A B  \<equiv> A \<and> \<not>B \<or> \<not>A \<and> B";
 
 text{*\noindent%
-where \isacommand{defs}\indexbold{*defs} is a keyword and
+where \commdx{defs} is a keyword and
 @{thm[source]nand_def} and @{thm[source]xor_def} are user-supplied names.
 The symbol \indexboldpos{\isasymequiv}{$IsaEq} is a special form of equality
 that must be used in constant definitions.
-Declarations and definitions can also be merged
+Declarations and definitions can also be merged in a \commdx{constdefs} 
+command: 
 *}
 
 constdefs nor :: gate
@@ -36,7 +37,7 @@ constdefs nor :: gate
           xor2 :: gate
          "xor2 A B \<equiv> (A \<or> B) \<and> (\<not>A \<or> \<not>B)";
 
-text{*\noindent\indexbold{*constdefs}%
-in which case the default name of each definition is $f$@{text"_def"}, where
+text{*\noindent
+The default name of each definition is $f$@{text"_def"}, where
 $f$ is the name of the defined constant.*}
 (*<*)end(*>*)
